## Recurrence examples

> Give asymptotic upper and lower bound for $T(n)$ in each of the following
> recurrences. Justify your answers.
>
> 1. $T(n) = 2T(n/2) + n^3$
> 2. $T(n) = T(8n/11) + n$
> 3. $T(n) = 16T(n/4) + n^2$
> 4. $T(n) = 4T(n/2) + n^2\lg n$
> 5. $T(n) = 8T(n/3) + n^2$
> 6. $T(n) = 7T(n/2) + n^2 \lg n$
> 7. $T(n) = 2T(n/4) + \sqrt{n}$
> 8. $T(n) = T(n - 2) + n^2$

1. $T(n) = 2T(n/2) + n^3 \in \Theta(n^3)$ (master method)
2. $T(n) = T(8n/11) + n \in \Theta(n)$ (master method, $\log_{11/8}1 = 0$)
3. $T(n) = 16T(n/4) + n^2 \in \Theta(n^2\lg{n})$ (master method)
4. $T(n) = 4T(n/2) + n^2\lg n \in \Theta(n^2\lg^2{n})$ (master method)
5. $T(n) = 8T(n/3) + n^2 \in \Theta(n^2)$ (master method, $\log_3 8 \le 2$)
6. $T(n) = 7T(n/2) + n^2 \lg n \in \Theta(n^{\lg 7})$ (master method, $\lg 7 >= 2 + \epsilon$)
7. $T(n) = 2T(n/4) + \sqrt{n} \in \Theta(\sqrt{n} \lg n)$ (master method)
8. $T(n) = T(n - 2) + n^2 \in \Theta(n^3)$ by the following:

$$ \begin{aligned}
   T(n) &= n^2 + T(n - 2) \\\\
   &= n^2 + (n - 2)^2 + T(n - 4) \\\\
   &= \sum_{i=0}^{n/2}(n -2i)^2 \\\\
   &= n^2 \sum_{i=0}^{n/2} 1 + 4 \sum_{i=0}^{n/2} i^2 - 4n \sum_{i=0}^{n/2} i \\\\
\end{aligned}$$

For the three sums above:

$$n^2 \sum_{i=0}^{n/2} 1 = \frac{n^3}{2}$$

$$4 \sum_{i=0}^{n/2} i^2 = \frac{4}{6} \left[\frac{n}{2}\left(\frac{n+2}{2}(n+1)\right)\right] = \frac{1}{3}(2n^3 + 6n^2 + 4n)$$

$$4n \sum_{i=0}^{n/2} i = 4n\left[\frac{1}{2}\frac{n}{2}\left(\frac{n+2}{2}\right)\right] = \frac{1}{2}(n^3 + 2n^2)$$

Now substitute back in these 3 simplifications:

$$ \begin{aligned}
   T(n) &= n^2 \sum_{i=0}^{n/2} 1 + 4 \sum_{i=0}^{n/2} i^2 - 4n \sum_{i=0}^{n/2} i \\\\
   &= \frac{n^3}{2} + \frac{1}{3}(2n^3 + 6n^2 + 4n) - \frac{1}{2}(n^3 + 2n^2) \\\\
   &= \frac{2}{3}n^3 + n^2 + \frac{4}{3}n \\\\
   &= \Theta(n^3)
\end{aligned}$$
