## Fibonacci numbers

> This problem develops properties of the Fibonacci numbers, which are defined
> by recurrence (3.22). We shall use the technique of generating functions to
> solve the Fibonacci recurrence. Define the generating function (or formal
> power series) $\mathcal{F}$ as
>
> $$ \begin{align}
>    \mathcal{F}(z) &= \sum_{i=0}^{\infty}F_iz^i \\\\
>                   &= 0 + z + z^2 + 2z^3 + 3z^4 + 5z^5 + 8z^6 + 13z^7 + 21z^8 + \ldots,
>    \end{align} $$
> where $F_i$ is the $i$th Fibonacci number.
>
> 1. Show that $\mathcal{F}(z) = z + z\mathcal{F}(z) + z^2\mathcal{F}$.
> 2. Show that
>    $$ \begin{align}
>       \mathcal{F}(z) &= \frac{z}{1 - z - z^2} \\\\
>                      &= \frac{z}{(1 - \phi z)(1 - \hat\phi z)} \\\\
>                      &= \frac{1}{\sqrt5}\Big(\frac{1}{1 - \phi z} - \frac{1}{1 - \hat{\phi} z}\Big)
>       \end{align} $$
>    where
>    $$ \phi = \frac{1 + \sqrt5}{2} = 1.61803\ldots \\\\
>       \hat\phi = \frac{1 - \sqrt5}{2} = -0.61803\ldots $$
> 3. Show that
>    $$ \mathcal{F}(z) = \sum_{i=0}^{\infty}\frac{1}{\sqrt5}(\phi^i - \hat{\phi}^i)z^i $$
> 4. Use part (c) to prove that $F_i = \phi^i / \sqrt5$ for $i > 0$, rounded to the nearest
>    integer. (Hint: Observe that $|\hat{\phi}| < 1$.)

### Part 1

$$ \begin{align}
   & z + z\mathcal{F}(z) + z^2\mathcal{F}(Z) = \\\\
   & = z + z\sum_{i=0}^{\infty}F_iz^i + z^2\sum_{i=0}^{\infty}F_iz^i \\\\
   & = z + \sum_{i=1}^{\infty}F_{i-1}z^i + \sum_{i=2}^{\infty}F_{i-2}z^i \\\\
   & = z + F_1z + \sum_{i=2}^{\infty}(F_{i-1} + F_{i-2})z^i \\\\
   & = z + F_1z + \sum_{i=2}^{\infty}F_iz^i \\\\
   & = \mathcal{F}(z)
   \end{align} $$

### Part 2

Let's just note that $\phi - \hat\phi = \sqrt5$,  $\phi + \hat\phi = 1$ and $\phi\hat\phi = - 1$ (just calculate them):

$$ \begin{align}
   \mathcal{F}(z) &= \frac{\mathcal{F}(z)(1 - z - z^2)}{1 - z - z^2} \\\\
        &= \frac{\mathcal{F}(z) - z\mathcal{F}(z) - z^2\mathcal{F}(z) - z + z}{1 - z - z^2} \\\\
        &= \frac{\mathcal{F}(z) - \mathcal{F}(z) + z}{1 - z - z^2} \\\\
        &= \frac{z}{1 - z - z^2} \\\\
        &= \frac{z}{1 - (\phi + \hat\phi)z + \phi\hat\phi z^2} \\\\
        &= \frac{z}{(1 - \phi z)(1 - \hat\phi z)} \\\\
        &= \frac{\sqrt5 z}{\sqrt5 (1 - \phi z)(1 - \hat\phi z)} \\\\
        &= \frac{(\phi - \hat\phi)z + 1 - 1}{\sqrt5 (1 - \phi z)(1 - \hat\phi z)} \\\\
        &= \frac{(1 - \hat\phi z) - (1 - \phi z)}{\sqrt5 (1 - \phi z)(1 - \hat\phi z)} \\\\
        &= \frac{1}{\sqrt5}\Big(\frac{1}{1 - \phi z} - \frac{1}{1 - \hat\phi z}\Big) \\\\
   \end{align} $$

### Part 3

We have that:

$$ \frac{1}{1 - x} = \sum_{k=0}^{\infty}x^k \quad\text{when } |x| < 1 $$

Thus:

$$ \begin{align}
   \mathcal{F}(n) &= \frac{1}{\sqrt5}\Big(\frac{1}{1 - \phi z} - \frac{1}{1 - \hat\phi z}\Big) \\\\
                  &= \frac{1}{\sqrt5}\Big(\sum_{i=0}^{\infty}\phi^i z^i - \sum_{i=0}^{\infty}\hat{\phi}^i z^i\Big) \\\\
                  &= \sum_{i=0}^{\infty}\frac{1}{\sqrt5}(\phi^i - \hat{\phi}^i) z^i
   \end{align} $$

### Part 4

$$ \mathcal{F}(z) = \sum_{i=0}^{\infty}\alpha_iz^i \quad\text{ where } \alpha_i = \frac{\phi^i - \hat{\phi}^i}{\sqrt5} $$

From this follows that $\alpha_i = F_i$, that is:

$$ F_i = \frac{\phi^i - \hat{\phi}^i}{\sqrt5}  = \frac{\phi^i}{\sqrt5} - \frac{\hat{\phi}^i}{\sqrt5} $$

For $i = 0$, $\phi/\sqrt5 = (\sqrt5 + 5)/10 > 0.5$. For $i > 2$, $|\hat{\phi}^i| < 0.5$.
