## Alternative quicksort analysis

> An alternative analysis of the running time of randomized quicksort focuses
> on the expected running time of each individual recursive call to
> `RANDOMIZED-QUICKSORT`, rather than on the number of comparisons performed. As
> in the analysis of Section 7.4.2, assume that the values of the elements are
> distinct.
>
> 1. Argue that, given an array of size $n$, the probability that any
>    particular element is chosen as the pivot is $1/n$. Use this to define
>    indicator random variables $X_i = I\\{i\text{th smallest element is chosen
>    as the pivot}\\}$. What is $\E[X_i]$?
> 2. Let $T(n)$ be a random variable denoting the running time of quicksort on
>    an array of size $n$. Argue that
>    $$ \E[T(n)] = \E\bigg[\sum_{q=1}^nX_q(T(q-1) + T(n-q) + \Theta(n))\bigg] \tag{7.2} $$
> 3. Show that we can rewrite equation (7.2) as
>    $$ \E[T(n)] = \frac{2}{n}\sum_{q=2}^{n-1}\E[T(q)] + \Theta(n) \tag{7.3} $$
> 4. Show that
>    $$ \sum_{q=1}^{n-1}q\lg{q} \le \frac{n^2}{2}\lg{n} - \frac{n^2}{8} \tag{7.4} $$
>    for $n \ge 2$. (<i>Hint</i>: Split the summation into two parts, one for $q
>    = 1, 2, 3, \ldots, \lceil n/2 \rceil - 1$ and one for $q = \lceil n/2 \rceil,
>    \ldots, n - 1$.
> 5. Using the bound from equation (7.4), show that the recurrence in equation
>    (7.3) has the solution $\E[T(n)] = \Theta(n\lg{n})$. (<i>Hint</i>: Show,
>    by substitution, that $\E[T(n)] \le an\lg{n}$ for sufficiently large $n$
>    and for some positive constant $a$.)

### Choosing a pivot

`PARTITION` is equally likely to pick any element as a pivot. Since there are
$n$ elements, the probability of one being picked is $1/n$. For the same
reason, $\E[X_i] = 1/n$.

### Running time of quicksort

Let the $q$th smallest element be the pivot. There are $n$ possible choices for
it, each with chance $X_q$. Each will solve the problem by breaking it down in
two parts of size $q - 1$ and $n - q$ and adding a linear factor. The formula
in (7.5) follows by the definition of expectation.

### The rewrite

$$ \begin{aligned}
   \E[T(n)] &= \E\bigg[\sum_{q=1}^nX_q(T(q-1) + T(n-q) + \Theta(n))\bigg] \\\\
            &= \sum_{q=1}^n\frac{1}{n}(\E[T(q-1)] + \E[T(n-q)] + \Theta(n))\bigg] \\\\
            &= \frac{1}{n}\sum_{q=1}^n\E[T(q-1)]
             + \frac{1}{n}\sum_{q=1}^n\E[T(n - q)]
             + \frac{1}{n}\sum_{q=1}^n\Theta(n) \\\\
            &= \frac{1}{n}\sum_{q=0}^{n-1}\E[T(q)]
             + \frac{1}{n}\sum_{q=0}^{n-1}\E[T(n - q + 1)]
             + \Theta(n) \\\\
            &= \frac{1}{n}\sum_{q=0}^{n-1}\E[T(q)]
             + \frac{1}{n}\sum_{q=0}^{n-1}\E[T(q)]
             + \Theta(n) \\\\
            &= \frac{2}{n}\sum_{q=0}^{n-1}\E[T(q)] + \Theta(n) \\\\
            &= \frac{2}{n}\sum_{q=2}^{n-1}\E[T(q)]
             + \frac{2\E[T(0)]}{n}
             + \frac{2\E[T(1)]}{n}
             + \Theta(n) \\\\
            &= \frac{2}{n}\sum_{q=2}^{n-1}\E[T(q)] + \Theta(n)
   \end{aligned} $$

### The bound

$$ \begin{aligned}
   \sum_{k=2}^{n-1}k\lg{k}
   &=   \sum_{k=2}^{\lceil n/2 \rceil - 1}k\lg{k} + \sum_{k=\lceil n/2 \rceil}^{n - 1}k\lg{k} \\\\
   &\le \sum_{k=2}^{n/2}k\lg{k} + \sum_{k=n/2 + 1}^{n}k\lg{k} \\\\
   &\le \sum_{k=2}^{n/2}k\lg(n/2) + \sum_{k=n/2 + 1}^{n}k\lg{n} \\\\
   &=   \lg(n/2)\sum_{k=2}^{n/2}k\ + \lg{n}\sum_{k=n/2 + 1}^{n}k \\\\
   &=   (\lg{n} - \lg{2})\bigg(\frac{(n/2)(n/2 + 1)}{2}\bigg) +
          \lg{n}\bigg(\frac{n(n+1)}{2} - \frac{(n/2)(n/2 + 1)}{2}\bigg) \\\\
   &=   \lg{n}\frac{n(n+1)}{2} - \frac{(n/2)(n/2 + 1)}{2} \\\\
   &=   \frac{1}{2}\lg{n}(n^2 + 2n + 1) - \frac{1}{8}(n^2 + 2n + 1/8) \\\\
   &=   \frac{1}{2}n^2\lg{n} - \frac{1}{8}n^2 - \frac{8n\lg{n} + 4\lg{n} - 2n - 1/8}{8} \\\\
   &\le \frac{1}{2}n^2\lg{n} - \frac{1}{8}n^2
   \end{aligned} $$

### The solution

We guess $\E[T(n)] \le an\lg{n}$:

$$ \begin{aligned}
   \E[T(n)] &=   \frac{2}{n}\sum_{q=2}^{n-1}\E[T(q)] + \Theta(n) \\\\
            &\le \frac{2}{n}\sum_{q=2}^{n-1}an\lg{n} + \Theta(n) & \text{(by the guess)} \\\\
            &\le \frac{2a}{n}\bigg(\frac{1}{2}n^2\lg{n} - \frac{1}{8}n^2\bigg)
                 + \Theta(n) & \text{(by 7.7)} \\\\
            &=   an\lg{n} - \frac{a}{4}n + \Theta(n) & \text{(by }\Theta\text{-notation)} \\\\
            &\le an\lg{n}
   \end{aligned} $$

Note that $\Theta$-notation allows us to pick $a$ and $n$ such that the last
derivation is possible.
