> Use the substitution method to show that each of the following recurrences
> defined on the reals has the asymptotic solution specified:
>
> 1. $T(n) = T(n - 1) + n$ has solution $T(n) = \O(n^2)$
> 2. $T(n) = T(n/2) + \Theta(1)$ has solution $T(n) = \O(\lg n)$
> 3. $T(n) = 2T(n/2) + n$ has solution $T(n) = \Theta(n \lg n)$
> 4. $T(n) = 2T(n/2 + 17) + n$ has solution $T(n) = \O(n \lg n)$
> 5. $T(n) = 2T(n/3) + \Theta(n)$ has solution $T(n) = \Theta(n)$
> 6. $T(n) = 4T(n/2) + \Theta(n)$ has solution $T(n) = \Theta(n^2)$

### a. $T(n) = T(n - 1) + n$

We guess $T(n) \le cn^2$ for a particular $c$. Then:

$$ T(n) \le c(n-1)^2 + n = cn^2 - 2cn + c + n$$

If we pick $c = 1$ we have:

$$ n^2 - 2n + 1 + n = n^2 - n + 1 \le n^2 \text{ for } n \ge 1 $$

### b. $T(n) = T(n/2) + \Theta(1)$

We guess $T(n) \le c\lg n$:

$$
  \begin{aligned}
  T(n) & \le c\lg(n/2) + \Theta(1) \\\\
       & = c\lg n - c \lg 2 + \Theta(1) \\\\
       & = c\lg n - c + \Theta(1) \\\\
       & \le c\lg n
  \end{aligned}
$$

As long as we pick $c$ to dominate $\Theta(1)$.

### c. $T(n) = 2T(n/2) + n$

First we guess $T(n) \le cn\lg{n}$:

$$ \begin{aligned}
   T(n) & = 2T(n/2) + n \\\\
        & \le 2c(n/2)\lg(n/2) + n \\\\
        & = cn\lg(n/2) + n \\\\
        & = cn\lg{n} - cn\lg{2} + n \\\\
        & = cn\lg{n} + (1 - c)n \\\\
        & \le cn\lg{n} \\\\
        & \text{for } c \ge 1
   \end{aligned} $$

Next we guess $T(n) \ge cn\lg n$:

$$ \begin{aligned}
   T(n) & = 2T(n/2) + n \\\\
        & \ge 2c(n/2)\lg(n/2) + n \\\\
        & = cn\lg n - cn\lg{2} + n \\\\
        & = cn\lg n + (1 - c)n \\\\
        & \ge cn\lg n \\\
        & \text{for } 0 < c \le 1
   \end{aligned} $$

### d. $T(n) = 2T(n/2 + 17) + n$

Let's guess $T(n) \le c(n-a)\lg(n-a)$:

$$ \begin{aligned}
   T(n) & \le 2c(\lfloor n/2 \rfloor + 17 - a)\lg(\lfloor n/2 \rfloor + 17 - a) + n \\\\
        & \le 2c(n/2 + 1 + 17 - a)\lg(n/2 + 1 + 17 - a) + n \\\\
        & \le c(n + 36 - 2a)\lg\frac{n + 36 - 2a}{2} + n \\\\
        & \le c(n + 36 - 2a)\lg(n + 36 - 2a) - c(n + 36 - 2a) + n & (c > 1, n > n_0 = f(a))\\\\
        & \le c(n + 36 - 2a)\lg(n + 36 - 2a) & (a \ge 36) \\\\
        & \le c(n - a)\lg(n - a)
   \end{aligned} $$

### e. $T(n) = 2T(n/3) + \Theta(n)$

To prove $\O$, we can guess $T(n) \le cn$:

$$ \begin{aligned}
   T(n) & = 2T(n/3) + \Theta(n) \\\\
        & \le 2c(n/3) + \Theta(n) \\\\
        & = cn - (1/3)cn + \Theta(n) \\\\
        & \le cn
   \end{aligned} $$

As long as we pick $c$ such that $c/3$ is enough to dominate $\Theta(n)$.

Proving for $\Omega$ is essentially the same with a different constant.

### f. $T(n) = 4T(n/2) + \Theta(n)$

To prove $\O$, we guess $T(n) \le cn^2 - dn$:


$$ \begin{aligned}
   T(n) & = 4T(n/2) + \Theta(n) \\\\
        & \le 4\big(c\frac{n^2}{4} - d\frac{n}{2}\big) + \Theta(n) \\\\
        & = cn^2 - 2dn + \Theta(n) \\\\
        & \le cn^2
   \end{aligned} $$

As long as we pick $d$ so $2dn$ dominates $\Theta(n)$. Proving $\Omega$ is super
similar.
