> The recurrence $T(n) = 2T(n - 1) + 1$ has the solution $T(n) = \O(2^n)$. Show
> that a substitution proof fails with the assumption $T(n) \le c2^n$, where
> $c > 0$ is constant. Then show how to subtract a lower-order term to make a
> substitution proof work.

So, let's start with guessing that $T(n) \le c2^n$:


$$ \begin{aligned}
     T(n) & = 2T(n - 1) + 1 \\\\
          & \le 2 c 2^{n-1} + 1 \\\\
          & = c2^n + 1
   \end{aligned} $$

No dice.

Let's guess instead that $T(n) \le c^2n - d$:

$$ \begin{aligned}
     T(n) & = 2T(n - 1) + 1 \\\\
          & \le 2 (c 2^{n-1} - d) + 1 \\\\
          & = c2^n - 2d + 1 \\\\
          & \le c2^n
   \end{aligned} $$

This holds, as long as we pick $d \ge 1/2$.
