> Using the master method in Section 4.5, you can show that the solution to
> the recurrence $T(n) = 4T(n/3) + n$ is $T(n) = \Theta(n^{\log_{3}4})$. Show
> that a substitution proof with the assumption $T(n) \leq cn^{\log_{3}4}$
> fails. Then show how to subtract off a lower-order term to make the
> substitution proof work.

First we guess $T(n) \le cn^{\log_3{4}}$. Thus:

$$ \begin{align}
   T(n) & \le 4c(n/3)^{\log_3{4}} + n \\\\
        & \le cn^{\log_3{4}} + n
   \end{align} $$

Dead-end!

Let's guess $T(n) \le cn^{\log_3{4}} - n$. Thus:

$$ \begin{align}
   T(n) & \le 4\Big(c(n/3)^{\log_3{4}} - n\Big) + n \\\\
        & \le cn^{\log_3{4}} - 4n + n \\\\
        & \le cn^{\log_3{4}} - 3n \\\\
        & \le cn^{\log_3{4}} - n
   \end{align} $$

We're done!
