> Prove the following:
>
> 1. Equation (3.21)
> 2. Equations (3.26)-(3.28)
> 3. $\lg(\Theta(n)) = \Theta(\lg n)$

Equation (3.21) is:

$$ a^{\log_bc} = c^{\log_ba} $$

We can prove it this way:

$$ \begin{aligned}
   a^{\log_bc} = a^{\frac{\log_ac}{\log_ab}} = \big(a^{\log_ac})^\frac{1}{\log_ab}
   = c^{\log_ba}
   \end{aligned} $$

---

The three equations are:

1. $n! = \omega(2^n)$
2. $n! = o(n^n)$
3. $\lg(n!) = \Theta(n\lg{n})$

The first two are kinda obvious:

$$
  \forall n > 3:
  2^n = \underbrace{2 \cdot 2 \cdot \cdots \cdot 2}_\text{n times} <
        1 \cdot 2 \cdot \cdots \cdot n = n!
        \quad\Rightarrow\quad n! = \omega(2^n)
$$

And:

$$
  \forall n > 1 :
  n! = 1 \cdot 2 \cdot \cdots n < \underbrace{n \cdot n \cdot \cdots \cdot n}_\text{n times}
     = n^n \quad \text{for }
     \quad\Rightarrow\quad n! = o(n^n)
$$

For the third, we use **Stirling's approximation**:

$$ \begin{aligned}
   \lg(n!) &= \lg\Bigg(\sqrt{2\pi{n}}\Big(\frac{n}{e}\Big)^n\Big(1+\Theta(\frac{1}{n})\Big)\Bigg)
      = \lg\sqrt{2\pi{n}} + \lg\Big(\frac{n}{e}\Big)^n + \lg\Big(1+\Theta(\frac{1}{n})\Big) = \\\\
     &= \Theta(\sqrt{n}) + n\lg{\frac{n}{e}} + \lg\Big(\Theta(1) + \Theta(\frac{1}{n})\Big)
      = \Theta(\sqrt{n}) + \Theta(n\lg{n}) + \Theta(\frac{1}{n}) = \\\\
     &= \Theta(n\lg{n})
   \end{aligned}
$$

---

We can prove the third subtask by doing $\Omega$ and $\O$ separately. Let's
start with $\O$. Because we have $\lg(\O(n))$, we know that there exists a
constant $c$ such that:

$$ \lg(\O(n)) \le \lg(cn) = \lg{c} + \lg{n} = \O(\lg{n}) $$

It works for $\Omega$ in the same way, but in the other direction (and a
different $c$).
