> Use the substitution method to prove that recurrence (4.14) has the solution
> $T(n) = \Theta(n\lg n)$. Conclude that $T(n) = \Theta(n \lg n)$.

Recurrence (4.14) is $T(n) = T(n/3) + T(2n/3) + \Theta(n)$. If we guess that
$T(n) \ge cn \lg n + dn$, we get:

$$
  \begin{aligned}
  T(n) & = T(n/3) + T(2n/3) + \Theta(n) \\\\
       & \ge \frac{1}{3}cn\lg{\frac{n}{3}} + \frac{1}{3}dn +
             \frac{2}{3}cn\lg{\frac{2n}{3}} + \frac{2}{3}dn +
             \Theta(n) \\\\
       & = \frac{1}{3}cn\lg{n} - \frac{1}{3}cn\lg{3} +
           \frac{2}{3}cn\lg{2} + \frac{2}{3}cn\lg{n} - \frac{2}{3}cn\lg{3} +
           dn + \Theta(n) \\\\
       & = cn\lg{n} + \frac{2}{3}cn - cn\lg{3} + dn + \Theta(n) \\\\
       & = cn\lg{n} + (d + \frac{2}{3} - \lg{3})cn + \Theta(n) \\\\
       & \ge cn\lg n
  \end{aligned}
$$

For the correct choice of $d$.
