> $\star$ For $f(n) = \Theta(n^{\log_b a}/\lg{n})$, prove that the summation in
> equation (4.19) has solution $g(n) = \Theta(n^{\log_b a}/\lg\lg{n})$. Conclude
> that a master recurrence $T(n)$ using $f(n)$ as its driving function has
> solution $T(n) = \Theta(n^{\log_b a}\lg\lg n)$.

Let's treat $\Theta(f(n))$ as $cf(n)$ for now. Substituting into equation
(4.19), we get:

$$
  \begin{aligned}
    g(n) & = \sum_{j=0}^{\lfloor \log_b{n} \rfloor} a^j f(n/b^j) \\\\
         & = \sum_{j=0}^{\lfloor \log_b{n} \rfloor} a^j
             c \Big(\frac{n}{b^j}\Big)^{\log_b{a}} \lg^{-1}(n/b^j) \\\\
         & = \sum_{j=0}^{\lfloor \log_b{n} \rfloor} a^j
             c \frac{n^{\log_b{a}}}{(b^j)^{\log_b{a}}} \lg^{-1}(n/b^j) \\\\
         & = \sum_{j=0}^{\lfloor \log_b{n} \rfloor} a^j
             c \frac{n^{\log_b{a}}}{a^j} \lg^{-1}(n/b^j) \\\\
         & = c n^{\log_b{a}} \sum_{j=0}^{\lfloor \log_b{n} \rfloor} \lg^{-1}(n/b^j)
  \end{aligned}
$$

We will now delve into the term under the sum. First note, that it's poorly
defined if $n / b^j = 1$, because it ends up as $1/\lg(1) = 1/0$. Rewriting
this, we know that $j \ne \log_b{n}$. We will (somehow) end up using that.

Going forward, let's explore the term:

$$ \begin{aligned}
   \lg^{-1}(n/b^j)
     & = \big( \lg(n/b^j) \big)^{-1} \\\\
     & = \Bigg( \frac{ \log_{b}(n/b^j) }{ \log_b{2} } \Bigg)^{-1} \\\\
     & = \log^{-1}_b(2) \big( \log_b{n} - \log_b{b^j} \big)^{-1} \\\\
     & = \lg(b) \big( \log_b{n} - j \big)^{-1} \\\\
     & = \lg(b) \frac{1}{ \log_b{n} - j} \\\\
   \end{aligned} $$

If we plug this back in, we get:

$$ \begin{aligned}
   g(n) & = c n^{\log_b{a}} \sum_{j=0}^{\lfloor \log_b{n} \rfloor} \lg(b) \frac{1}{ \log_b{n} - j} \\\\
        & = c \lg(b) n^{\log_b{a}} \sum_{j=0}^{\lfloor \log_b{n} \rfloor} \frac{1}{ \log_b{n} - j} \\\\
   \end{aligned} $$

We will now hand-wave, and ignore both the floor and the fact that $j$ doesn't
go up to $\log_{b}{n}$, two things that we'll pretend cancel each other. After
we reindex, we get:

$$ \begin{aligned}
   g(n) & = c \lg(b) n^{\log_b{a}} \sum_{j=0}^{\log_b{n}} \frac{1}{ \log_b{n} - j} \\\\
        & = c \lg(b) n^{\log_b{a}} \sum_{k=0}^{\log_b{n}} \frac{1}{k} \\\\
   \end{aligned} $$

We also know this $k$ is not going to be $0$ (because $j$ can't be $\log_b n$)
and we will just ignore it, to get:

$$ g(n) = c \lg(b) n^{\log_b{a}} \sum_{k=1}^{\log_b{n}} \frac{1}{k} $$

This now leaves us with the harmonic series, in order to get:

$$ g(n) = c \lg(b) n^{\log_b{a}} \big( \ln{\log_b{n}} + \Theta(1) \big) $$

We hand-wave a bit more to rebase the logarithm:

$$
  \ln\log_b{n} = \frac{ \lg\log_b n}{ \lg e }
               = \lg^{-1}(e) \cdot \frac{ \lg n }{ \lg b }
               = \lg^{-1}(e) \big( \lg\lg n - \lg\lg b \big)
               = \Theta(\lg\lg n)
$$

Plugging that back in, we get:

$$
  g(n) = c \lg(b) n^{\log_b{a}} \big( \Theta(\lg\lg n) + \Theta(1) \big)
       = \Theta(n^{\log_b a}\lg\lg n)
$$

And we're done, if we pretend that this was rigorous enough.
