## Alternative analysis of randomized selection

> In this problem, we use indicator random variables to analyze the
> `RANDOMIZED-SELECT` procedure in a manner akin to our analysis of
> `RANDOMIZED-QUICKSORT` in section 7.4.2.
>
> As in the quicksort analysis, we assume that all the elements are distinct,
> and we rename the elements of the input array $A$ as $z_1, z_2, \ldots,
> z_n$, where $z_i$ is the $i$th smallest element. Thus, the call
> `RANDOMIZED-SELECT(A,1,n,k)` returns $z_k$.
>
> For $i \le i < j \le n$, let
>
> $$ X_{ijk} = I\\{z_i \text{ is compared with } z_j \text{ sometime during
>    the execution of the algorithm to find } z_k \\} $$
>
> <ol type="a">
>   <li>Give an exact expression for $\E[X_{ijk}]$. (<i>Hint:</i> Your
>   expression may have different values, depending on the values of $i$, $j$,
>   and $k$.)
>   <li>Let $X_k$ denote the total number of comparisons between elements of
>   array $A$ when finding $z_k$. Show that
>   $$ \E[X_k] \le 2 \bigg(
>        \sum_{i=1}^k \sum_{j=k}^n \frac{1}{j - i + 1} +
>        \sum_{j=k+1}^n \frac{j - k - 1}{j - k + 1} +
>        \sum_{i=1}^{k-2} \frac{k - i - 1}{k - i + 1}
>        \bigg) $$
>   <li>Show that $\E[X_k] \le 4n$.
>   <li>Conclude that, assuming all elements of array $A$ are distinct,
>   `RANDOMIZED-SELECT` runs in expected time $\O(n)$.
> </ol>

### Expectation of exchanging two elements

The situation is very similar to the quicksort analysis, although $k$ matters.
$z_i$ and $z_j$ will be compared if one of them is the first element to get
picked as a pivot in the smallest interval containing $i$, $j$ and $k$. The
exact expression depends on the position of $k$ in regards to the other two:

$$ \E[X_{ijk}] =
     \begin{cases}
       2 / (k - i + 1) & \text{if } i < j \le k \\\\
       2 / (j - i + 1) & \text{if } i \le k \le j \\\\
       2 / (j - k + 1) & \text{if } k \le i < j
     \end{cases}
$$

### The expected number of comparisons

It's a long derivation:

$$ \begin{align}
   \E[X_k] &= \sum_{i=1}^{n-1}   \sum_{j=i+1}^n \E[X_{ijk}] \\\\
           &= \sum_{i=1}^k       \sum_{j=i+1}^n \E[X_{ijk}]
            + \sum_{i=k+1}^{n-1} \sum_{j=i+1}^n \E[X_{ijk}] \\\\
           &= \sum_{i=1}^k \bigg(\sum_{j=i+1}^{k-1}\E[X_{ijk}]
                                 + \sum_{j=k}^n\E[X_{ijk}] \bigg)
            + \sum_{i=k+1}^{n-1}\sum_{j=i+1}^n\E[X_{ijk}] \\\\
           &= \sum_{i=1}^k       \sum_{j=i+1}^{k-1} \E[X_{ijk}]
            + \sum_{i=1}^k       \sum_{j=k}^n       \E[X_{ijk}]
            + \sum_{i=k+1}^{n-1} \sum_{j=i+1}^n     \E[X_{ijk}] \\\\
           &= \sum_{i=1}^{k-2}   \sum_{j=i+1}^{k-1} \E[X_{ijk}]
            + \sum_{i=1}^k       \sum_{j=k}^n       \E[X_{ijk}]
            + \sum_{i=k+1}^{n-1} \sum_{j=i+1}^n     \E[X_{ijk}] \\\\
           &= \sum_{i=1}^{k-2}   \sum_{j=i+1}^{k-1} \frac{2}{k - i + 1}
            + \sum_{i=1}^k       \sum_{j=k}^n       \frac{2}{j - i + 1}
            + \sum_{i=k+1}^{n-1} \sum_{j=i+1}^n     \frac{2}{j - k + 1} \\\\
           &= 2\bigg(
                \sum_{i=1}^k       \sum_{j=k}^n       \frac{1}{j - i + 1}
              + \sum_{i=k+1}^{n-1} \sum_{j=i+1}^n     \frac{1}{j - k + 1}
              + \sum_{i=1}^{k-2}   \sum_{j=i+1}^{k-1} \frac{1}{k - i + 1}
              \bigg) \\\\
           &= 2\bigg(
                \sum_{i=1}^k       \sum_{j=k}^n       \frac{1}{j - i + 1}
              + \sum_{i=k+1}^{n-1} \sum_{j=i+1}^n     \frac{1}{j - k + 1}
              + \sum_{i=1}^{k-2}   \frac{k - i - 1}{k - i + 1}
              \bigg) \\\\
           &= 2\bigg(
                \sum_{i=1}^k       \sum_{j=k}^n       \frac{1}{j - i + 1}
              + \sum_{j=k+2}^n     \sum_{i=k+1}^{j-1} \frac{1}{j - k + 1}
              + \sum_{i=1}^{k-2}   \frac{k - i - 1}{k - i + 1}
              \bigg) & \text{(note below)} \\\\
           &= 2\bigg(
                \sum_{i=1}^k       \sum_{j=k}^n       \frac{1}{j - i + 1}
              + \sum_{j=k+2}^n     \frac{j - k - 1}{j - k + 1}
              + \sum_{i=1}^{k-2}   \frac{k - i - 1}{k - i + 1}
              \bigg) \\\\
           &\le 2\bigg(
                \sum_{i=1}^k       \sum_{j=k}^n       \frac{1}{j - i + 1}
              + \sum_{j=k+1}^n     \frac{j - k - 1}{j - k + 1}
              + \sum_{i=1}^{k-2}   \frac{k - i - 1}{k - i + 1}
              \bigg) \\\\
   \end{align} $$

The last noted derivation is valid because of the following iversonian
equation:

$$ [k+1 \le i \le n - 1][i+1 \le j \le n] =
   [k+1 \le i < i + 1 < j \le n] =
   [k + 1 < j \le n][k + 1 \le i < j]$$

Concrete mathematics helped a lot!

### Bounding to 4n

Let's take the expressions in parts. The last two are straightforward enough:

$$ \sum_{j=k+1}^n\frac{j-k-1}{j-k+1} + \sum_{i=1}^{k-2}\frac{k-i-1}{k-i+1}
   \le \sum_{j=k+1}^n 1 + \sum_{i=1}^{k-2} 1
   = n - k + k - 2
   \le n $$

This one is a bit trickier for me:

$$ \sum_{i=1}^k \sum_{j=k}^n \frac{1}{j - i + 1} $$

It contains terms of the form $1/m$ where $1 \le m \le n$. It contains $1/1$
at most once, $1/2$ at most twice, $1/3$ at most three times and so on. Thus,
the sum of the expressions $1/m$ for each $m$ is at most $1$ and there are $n$
such different expressions, which bounds the whole sum to $n$.

There should be a way to manipulate the sums to prove that, but I cannot find
it. In any case, both expressions are at most $2n$, which means that $\E[X_k]
\le 4n$.

### Conclusion

Well, it's rather obvious, isn't it? The number of operations in
`RANDOMIZED-SELECT` are linear to the number of comparisons, and the expected
number of comparisons are bound by a linear function, which means that the
expected running time is linear.
